Revert changes relating to instance generation
Revert "Add todo for missing logic around instantiations"
This reverts commit 303a45374643f75698c61f062899973d2c297831.

Revert "Add wires and use them for output of instances"
This reverts commit a72f26319dabca414a2b576424b9f72afaca161c.

Revert "Separate HTL instantiations from Verilog ones"
This reverts commit 653c8729f4322f538aa7116c5e311c884b3c5047.

Revert "Translate instantiations from HTL to verilog"
This reverts commit 982e6c69a52e8ec4e677147004cc5472f8a80d6d.

Revert "Print instantiations in HTL output"
This reverts commit 9b87637d3e4d6a75dee1221b017e3ccf6632642e.

Revert "Add a field in HTL modules for instances"
This reverts commit d79dae026b150e9671e0aa7262f6aa2d1d302502.

Revert "Generate (invalid) module instantiations for calls"
This reverts commit dfaa3a9cbc07649feea3220693a8a854a32eafb6.

src/verilog/PrintHTL.ml
@@ -31,7 +31,6 @@ open VericertClflags
 
 let pstr pp = fprintf pp "%s"
 
-(* TODO import from PrintVerilog.v *)
 let rec intersperse c = function
   | [] -> []
   | [x] -> [x]
@@ -39,14 +38,9 @@ let rec intersperse c = function
 
 let register a = sprintf "reg_%d" (P.to_int a)
 let registers a = String.concat "" (intersperse ", " (List.map register a))
-let vmodule a = sprintf "%s" (extern_atom a)
-let instance a = sprintf "instance_%d" (P.to_int a)
 
 let print_instruction pp (pc, i) =
   fprintf pp "%5d:\t%s" pc (pprint_stmnt 0 i)
-
-let print_instantiation pp (pc, HTLinstantiation (mod_name, inst_name, args, dst, fin)) =
-  fprintf pp "%5d:\t %s %s(%s) -> %s\n" pc (vmodule mod_name) (instance inst_name) (registers args) (register dst)
 
 let ptree_to_list ptree =
   List.sort
@@ -59,12 +53,6 @@ let print_module pp id f =
   fprintf pp "%s(%s) {\n" (extern_atom id) (registers f.mod_params);
   let datapath = ptree_to_list f.mod_datapath in
   let controllogic = ptree_to_list f.mod_controllogic in
-  let insts = ptree_to_list f.mod_insts in
-  if List.length insts > 0 then (
-    fprintf pp "  instances {\n";
-    List.iter (print_instantiation pp) insts;
-    fprintf pp "  }\n\n";
-  ) else fprintf pp "  ";
   fprintf pp "datapath {\n";
   List.iter (print_instruction pp) datapath;
   fprintf pp "  }\n\n  controllogic {\n";
