src/Compiler.v
@@ -82,6 +82,7 @@ Qed.
 
 Definition transf_backend (r : RTL.program) : res Verilog.program :=
   OK r
+  @@@ Inlining.transf_program
   @@ print (print_RTL 1)
   @@@ HTLgen.transl_program
   @@ print print_HTL
@@ -143,8 +144,8 @@ Proof.
   exists p7; split. apply Inliningproof.transf_program_match; auto.
   exists p8; split. apply HTLgenproof.transf_program_match; auto.
   exists p9; split. apply Veriloggenproof.transf_program_match; auto.
-  inv T. (* reflexivity. *)
-Admitted.
+  inv T. reflexivity.
+Qed.
 
 Remark forward_simulation_identity:
   forall sem, forward_simulation sem sem.
