src/verilog/Verilog.v
@@ -39,7 +39,6 @@ Set Implicit Arguments.
 
 Definition reg : Type := positive.
 Definition node : Type := positive.
-Definition ident : Type := positive.
 Definition szreg : Type := reg * nat.
 
 Record associations (A : Type) : Type :=
@@ -100,15 +99,7 @@ Definition block_reg (r : reg) (asr : reg_associations) (v : value) :=
 Definition nonblock_reg (r : reg) (asr : reg_associations) (v : value) :=
   mkassociations asr.(assoc_blocking) (AssocMap.set r v asr.(assoc_nonblocking)).
 
-Inductive io : Type :=
-| Vinput : io
-| Voutput : io
-| Vinout : io.
-
-Inductive scl_decl : Type :=
-| VScalar (io: option Verilog.io) (sz : nat)
-| VWire (sz : nat).
-
+Inductive scl_decl : Type := VScalar (sz : nat).
 Inductive arr_decl : Type := VArray (sz : nat) (ln : nat).
 
 (** * Verilog AST
@@ -202,13 +193,18 @@ Inductive edge : Type :=
 
 (** ** Module Items
 
-Module items can either be declarations ([Vdecl]) or always blocks ([Valways]). *)
+Module items can either be declarations ([Vdecl]) or always blocks ([Valways]).
+The declarations are always register declarations as combinational logic can be
+done using combinational always block instead of continuous assignments. *)
+
+Inductive io : Type :=
+| Vinput : io
+| Voutput : io
+| Vinout : io.
 
 Inductive declaration : Type :=
 | Vdecl : option io -> reg -> nat -> declaration
-| Vdeclarr : option io -> reg -> nat -> nat -> declaration
-| Vdeclwire : reg -> nat -> declaration
-| Vinstancedecl : ident -> ident -> list reg -> declaration.
+| Vdeclarr : option io -> reg -> nat -> nat -> declaration.
 
 Inductive module_item : Type :=
 | Vdeclaration : declaration -> module_item
